IsaSAT: use stamping for lbd instead of cleaning each time
Previously, an array of bools was used that had to be emptied each
time after marking another clause. We now use a stamp (a natural
number): The value is present iff we have stamp at the position.
Cleaning is very cheap most of the time (increment stamp) and
expensive before overflowing. This is an obvious and trivial
improvement.

Weidenbach_Book/IsaSAT/LBD.thy
@@ -20,20 +20,22 @@ Remark that we combine the LBD with a MTF scheme.
 
 section \<open>Types and relations\<close>
 type_synonym lbd = \<open>bool list\<close>
-type_synonym lbd_ref = \<open>bool list \<times> nat \<times> nat\<close>
+type_synonym lbd_ref = \<open>nat list \<times> nat \<times> nat\<close>
 
 
 text \<open>Beside the actual ``lookup'' table, we also keep the highest level marked so far to unmark
 all levels faster (but we currently don't save the LBD and have to iterate over the data structure).
-We also handle growing of the structure by hand instead of using a proper hash-table. We do so,
-because there are much stronger guarantees on the key that there is in a general hash-table
-(especially, our numbers are all small).
+We also handle growing of the structure by hand instead of using a proper hash-table.
 \<close>
-definition lbd_ref where
-  \<open>lbd_ref = {((lbd, n, m), lbd'). lbd = lbd' \<and> n < length lbd \<and>
-      (\<forall>k > n. k < length lbd \<longrightarrow> \<not>lbd!k) \<and>
-      length lbd \<le> Suc (Suc (uint32_max div 2)) \<and> n < length lbd \<and>
-      m = length (filter id lbd)}\<close>
+definition lbd_ref :: \<open>(lbd_ref \<times> lbd) set\<close> where
+  \<open>lbd_ref = {((lbd, stamp, m), lbd').
+      length lbd' \<le> Suc (Suc (uint32_max div 2)) \<and>
+      m = length (filter id lbd') \<and>
+      stamp > 0 \<and>
+      length lbd = length lbd' \<and>
+     (\<forall>v \<in> set lbd. v \<le> stamp) \<and>
+     (\<forall>i < length lbd'. lbd' ! i \<longleftrightarrow>  lbd ! i = stamp)
+}\<close>
 
 
 section \<open>Testing if a level is marked\<close>
@@ -42,7 +44,7 @@ definition level_in_lbd :: \<open>nat \<Rightarrow> lbd \<Rightarrow> bool\<clos
   \<open>level_in_lbd i = (\<lambda>lbd. i < length lbd \<and> lbd!i)\<close>
 
 definition level_in_lbd_ref :: \<open>nat \<Rightarrow> lbd_ref \<Rightarrow> bool\<close> where
-  \<open>level_in_lbd_ref = (\<lambda>i (lbd, _). i < length_uint32_nat lbd \<and> lbd!i)\<close>
+  \<open>level_in_lbd_ref = (\<lambda>i (lbd, stamp, _). i < length_uint32_nat lbd \<and> lbd!i = stamp)\<close>
 
 lemma level_in_lbd_ref_level_in_lbd:
   \<open>(uncurry (RETURN oo level_in_lbd_ref), uncurry (RETURN oo level_in_lbd)) \<in>
@@ -60,14 +62,14 @@ definition lbd_write :: \<open>lbd \<Rightarrow> nat \<Rightarrow> lbd\<close> w
 
 
 definition lbd_ref_write :: \<open>lbd_ref \<Rightarrow> nat \<Rightarrow> lbd_ref nres\<close>  where
-  \<open>lbd_ref_write = (\<lambda>(lbd, m, n) i. do {
+  \<open>lbd_ref_write = (\<lambda>(lbd, stamp, n) i. do {
     ASSERT(length lbd \<le> uint32_max \<and> n + 1 \<le> uint32_max);
     (if i < length_uint32_nat lbd then
-       let n = if lbd ! i then n else n+1 in
-       RETURN (lbd[i := True], max i m, n)
+       let n = if lbd ! i = stamp then n else n+1 in
+       RETURN (lbd[i := stamp], stamp, n)
      else do {
         ASSERT(i + 1 \<le> uint32_max);
-        RETURN ((list_grow lbd (i + 1) False)[i := True], max i m, n + 1)
+        RETURN ((list_grow lbd (i + 1) 0)[i := stamp], stamp, n + 1)
      })
   })\<close>
 
@@ -87,90 +89,78 @@ lemma lbd_ref_write_lbd_write:
     (auto simp: level_in_lbd_ref_def level_in_lbd_def lbd_ref_def list_grow_def
         nth_append uint32_max_def length_filter_update_true list_update_append2
         length_filter_update_false
-      intro!: ASSERT_leI le_trans[OF length_filter_le])
+      intro!: ASSERT_leI le_trans[OF length_filter_le]
+      elim!: in_set_upd_cases)
+
 
 section \<open>Cleaning the marked levels\<close>
 
-definition lbd_emtpy_inv :: \<open>nat \<Rightarrow> bool list \<times> nat \<Rightarrow> bool\<close> where
-  \<open>lbd_emtpy_inv m = (\<lambda>(xs, i). i \<le> Suc m \<and> (\<forall>j < i. xs ! j = False) \<and>
-    (\<forall>j > m. j < length xs \<longrightarrow> xs ! j = False))\<close>
+definition lbd_emtpy_inv :: \<open>nat list \<Rightarrow> nat list \<times> nat \<Rightarrow> bool\<close> where
+  \<open>lbd_emtpy_inv ys = (\<lambda>(xs, i). (\<forall>j < i. xs ! j = 0) \<and> i \<le> length xs \<and> length ys = length xs)\<close>
 
-definition lbd_empty_ref where
-  \<open>lbd_empty_ref = (\<lambda>(xs, m, _). do {
+definition lbd_empty_loop_ref where
+  \<open>lbd_empty_loop_ref = (\<lambda>(xs, _, _). do {
     (xs, i) \<leftarrow>
-       WHILE\<^sub>T\<^bsup>lbd_emtpy_inv m\<^esup>
-         (\<lambda>(xs, i). i \<le> m)
+       WHILE\<^sub>T\<^bsup>lbd_emtpy_inv xs\<^esup>
+         (\<lambda>(xs, i). i < length xs)
          (\<lambda>(xs, i). do {
             ASSERT(i < length xs);
             ASSERT(i + 1 < uint32_max);
-            RETURN (xs[i := False], i + 1)})
+            RETURN (xs[i := 0], i + 1)})
          (xs, 0);
-     RETURN (xs, 0, 0)
+     RETURN (xs, 1, 0)
   })\<close>
 
 definition lbd_empty where
    \<open>lbd_empty xs = RETURN (replicate (length xs) False)\<close>
 
-lemma lbd_empty_ref:
-  assumes \<open>((xs, m, n), xs) \<in> lbd_ref\<close>
+lemma lbd_empty_loop_ref:
+  assumes \<open>((xs, m, n), ys) \<in> lbd_ref\<close>
   shows
-    \<open>lbd_empty_ref (xs, m, n) \<le> \<Down> lbd_ref (RETURN (replicate (length xs) False))\<close>
+    \<open>lbd_empty_loop_ref (xs, m, n) \<le> \<Down> lbd_ref (RETURN (replicate (length ys) False))\<close>
 proof -
-  have m_xs: \<open>m \<le> length xs\<close> and [simp]: \<open>xs \<noteq> []\<close> and le_xs: \<open>length xs \<le> uint32_max div 2 + 2\<close>
+  have le_xs: \<open>length xs \<le> uint32_max div 2 + 2\<close>
+    \<open>length ys = length xs\<close>
     using assms by (auto simp: lbd_ref_def)
   have [iff]: \<open>(\<forall>j. \<not> j < (b :: nat)) \<longleftrightarrow> b = 0\<close> for b
     by auto
-  have init: \<open>lbd_emtpy_inv m (xs, 0)\<close>
-    using assms m_xs unfolding lbd_emtpy_inv_def
+  have init: \<open>lbd_emtpy_inv xs (xs, 0)\<close>
+    unfolding lbd_emtpy_inv_def
     by (auto simp: lbd_ref_def)
-  have lbd_remove: \<open>lbd_emtpy_inv m
-       (a[b := False], b + 1)\<close>
+  have lbd_remove: \<open>lbd_emtpy_inv xs (a[b := 0], b + 1)\<close>
     if
-      inv: \<open>lbd_emtpy_inv m s\<close> and
+      inv: \<open>lbd_emtpy_inv xs s\<close> and
       \<open>case s of (ys, i) \<Rightarrow> length ys = length xs\<close> and
-      cond: \<open>case s of (xs, i) \<Rightarrow> i \<le> m\<close> and
+      cond: \<open>case s of (xs, i) \<Rightarrow> i < length xs\<close> and
       s: \<open>s = (a, b)\<close> and
-      [simp]: \<open>b < length a\<close>
+      b_le: \<open>b < length a\<close>
     for s a b
   proof -
-    have 1: \<open>a[b := False] ! j = False\<close> if \<open>j<b\<close> for j
+    have 1: \<open>a[b := 0] ! j = 0\<close> if \<open>j<b\<close> for j
       using inv that unfolding lbd_emtpy_inv_def s
       by auto
-    have 2: \<open>\<forall>j>m. j < length (a[b := False]) \<longrightarrow> a[b := False] ! j = False\<close>
-      using inv that unfolding lbd_emtpy_inv_def s
-      by auto
-    have \<open>b + 1 \<le> Suc m\<close>
-      using cond unfolding s by simp
-    moreover have \<open>a[b := False] ! j = False\<close> if \<open>j<b + 1\<close> for j
-      using 1[of j] that cond by (cases \<open>j = b\<close>) auto
-    moreover have \<open>\<forall>j>m. j < length (a[b := False]) \<longrightarrow> a[b := False] ! j = False\<close>
-      using 2 by auto
-    ultimately show ?thesis
-      unfolding lbd_emtpy_inv_def by auto
+    have \<open>a[b := 0] ! j = 0\<close> if \<open>j<b + 1\<close> for j
+      using 1[of j] that cond b_le by (cases \<open>j = b\<close>) auto
+    then show ?thesis
+      using cond inv unfolding lbd_emtpy_inv_def s by auto
   qed
-  have lbd_final: \<open>((a, 0, 0), replicate (length xs) False) \<in> lbd_ref\<close>
+  have lbd_final: \<open>((a, 1, 0), replicate (length ys) False) \<in> lbd_ref\<close>
     if
-      lbd: \<open>lbd_emtpy_inv m s\<close> and
+      lbd: \<open>lbd_emtpy_inv xs s\<close> and
       I': \<open>case s of (ys, i) \<Rightarrow> length ys = length xs\<close> and
-      cond: \<open>\<not> (case s of (xs, i) \<Rightarrow> i \<le> m)\<close> and
+      cond: \<open>\<not> (case s of (xs, i) \<Rightarrow> i < length xs)\<close> and
       s: \<open>s = (a, b)\<close>
       for s a b
   proof -
-    have 1: \<open>a[b := False] ! j = False\<close> if \<open>j<b\<close> for j
-      using lbd that unfolding lbd_emtpy_inv_def s
-      by auto
-    have 2: \<open>j>m \<longrightarrow> j < length a \<longrightarrow> a ! j = False\<close> for j
+    have 1: \<open>a[b := 0] ! j = 0\<close> if \<open>j<b\<close> for j
       using lbd that unfolding lbd_emtpy_inv_def s
       by auto
     have [simp]: \<open>length a = length xs\<close>
       using I' unfolding s by auto
-    have [simp]: \<open>b = Suc m\<close>
-      using cond lbd unfolding lbd_emtpy_inv_def s
-      by auto
-    have [dest]: \<open>i < length xs \<Longrightarrow> \<not>a ! i\<close> for i
-      using 1[of i] 2[of i] by (cases \<open>i < Suc m\<close>) auto
+    have [dest]: \<open>i < length xs \<Longrightarrow> a ! i = 0\<close> for i
+      using 1[of i] lbd cond unfolding s lbd_emtpy_inv_def by (cases \<open>i < Suc m\<close>) auto
 
-    have [simp]: \<open>a = replicate (length xs) False\<close>
+    have [simp]: \<open>a = replicate (length xs) 0\<close>
       unfolding list_eq_iff_nth_eq
       apply (intro conjI)
       subgoal by simp
@@ -180,21 +170,42 @@ proof -
       using le_xs by (auto simp: lbd_ref_def)
   qed
   show ?thesis
-    unfolding lbd_empty_ref_def conc_fun_RETURN
+    unfolding lbd_empty_loop_ref_def conc_fun_RETURN
     apply clarify
-    apply (refine_vcg WHILEIT_rule_stronger_inv[where R = \<open>measure (\<lambda>(xs, i). Suc m - i)\<close> and
+    apply (refine_vcg WHILEIT_rule_stronger_inv[where R = \<open>measure (\<lambda>(xs, i). length xs - i)\<close> and
       I' = \<open>\<lambda>(ys, i). length ys = length xs\<close>])
     subgoal by auto
     subgoal by (rule init)
     subgoal by auto
-    subgoal using assms by (auto simp: lbd_ref_def)
-    subgoal using m_xs le_xs by (auto simp: uint32_max_def)
+    subgoal by auto
+    subgoal using assms by (auto simp: lbd_ref_def lbd_emtpy_inv_def uint32_max_def)
     subgoal by (rule lbd_remove)
     subgoal by auto
-    subgoal by auto
+    subgoal by (auto simp: lbd_emtpy_inv_def)
     subgoal by (rule lbd_final)
     done
 qed
+
+definition lbd_empty_cheap_ref where
+  \<open>lbd_empty_cheap_ref = (\<lambda>(xs, stamp, n). RETURN (xs, stamp + 1, 0))\<close>
+
+lemma lbd_empty_cheap_ref:
+  assumes \<open>((xs, m, n), ys) \<in> lbd_ref\<close>
+  shows
+    \<open>lbd_empty_cheap_ref (xs, m, n) \<le> \<Down> lbd_ref (RETURN (replicate (length ys) False))\<close>
+  using assms unfolding lbd_empty_cheap_ref_def lbd_ref_def
+  by (auto simp: filter_empty_conv all_set_conv_nth in_set_conv_nth)
+
+definition lbd_empty_ref :: \<open>lbd_ref \<Rightarrow>  lbd_ref nres\<close> where
+  \<open>lbd_empty_ref = (\<lambda>(xs, m, n). if m = uint32_max then lbd_empty_loop_ref (xs,m,n)
+    else lbd_empty_cheap_ref (xs, m, n)) \<close>
+
+lemma lbd_empty_ref:
+  assumes \<open>((xs, m, n), ys) \<in> lbd_ref\<close>
+  shows
+    \<open>lbd_empty_ref (xs, m, n) \<le> \<Down> lbd_ref (RETURN (replicate (length ys) False))\<close>
+  using lbd_empty_cheap_ref[OF assms] lbd_empty_loop_ref[OF assms]
+  by (auto simp: lbd_empty_ref_def)
 
 lemma lbd_empty_ref_lbd_empty:
   \<open>(lbd_empty_ref, lbd_empty) \<in> lbd_ref \<rightarrow>\<^sub>f \<langle>lbd_ref\<rangle>nres_rel\<close>
@@ -202,19 +213,20 @@ lemma lbd_empty_ref_lbd_empty:
   apply clarify
   subgoal for lbd m lbd'
     using lbd_empty_ref[of lbd m]
-    by (auto simp: lbd_empty_def lbd_ref_def)
+    by (auto simp: lbd_empty_def)
   done
 
 definition (in -)empty_lbd :: \<open>lbd\<close> where
    \<open>empty_lbd = (replicate 32 False)\<close>
 
 definition empty_lbd_ref :: \<open>lbd_ref\<close> where
-   \<open>empty_lbd_ref = (replicate 32 False, 0, 0)\<close>
+   \<open>empty_lbd_ref = (replicate 32 0, 1, 0)\<close>
 
 lemma empty_lbd_ref_empty_lbd:
   \<open>(\<lambda>_. (RETURN empty_lbd_ref), \<lambda>_. (RETURN empty_lbd)) \<in> unit_rel \<rightarrow>\<^sub>f \<langle>lbd_ref\<rangle>nres_rel\<close>
   by (intro frefI nres_relI) (auto simp: empty_lbd_def lbd_ref_def empty_lbd_ref_def
       uint32_max_def nth_Cons split: nat.splits)
+
 
 section \<open>Extracting the LBD\<close>
 
